removing an assume in Impl.Poly1305_64

code/poly1305/Hacl.Impl.Poly1305_64.fst
@@ -551,8 +551,11 @@ let poly1305_finish_ log st mac m len key_s =
   cut (disjoint acc mac);
   let h2 = ST.get() in
   no_upd_lemma_1 h0 h2 acc key_s;
+  assert (equal h0 key_s h2 key_s);
   let k'  = hload128_le key_s in
-  (* cut *) assume (k' == Hacl.Spec.Poly1305_64.load128_le_spec (as_seq h0 key_s)); //NS: Used to be a "cut"; But, now without this targetted assume, Z3-4.5.1 takes forever;
+  assert (FStar.UInt128.v k' == FStar.Endianness.little_endian (as_seq h0 key_s));
+  FStar.UInt128.v_inj k' (FStar.UInt128.uint_to_t (FStar.Endianness.little_endian (as_seq h0 key_s))); //NS: 07/14 ... need to invoke injectivity explicitly; which is rather heavy
+  assert (k' == Hacl.Spec.Poly1305_64.load128_le_spec (as_seq h0 key_s));
   let open Hacl.Bignum.Wide in
   let acc' = bignum_to_128 acc in
   let mac' = acc' +%^ k' in
